ulib/LowStar.RST.Pointer.fst
@@ -26,13 +26,13 @@ open LowStar.RST
 
 open LowStar.BufferOps
 
-(* Pointer view and resource *)
+(* View and resource for (heap-allocated, freeable) pointer resources *)
 
 abstract
 let ptr_view (#a:Type) (ptr:B.pointer a) : view a = 
   reveal_view ();
-  let fp = Ghost.hide (B.loc_buffer ptr) in 
-  let inv h = B.live h ptr in
+  let fp = Ghost.hide (B.loc_addr_of_buffer ptr) in 
+  let inv h = B.live h ptr /\ B.freeable ptr in
   let sel h = Seq.index (B.as_seq h ptr) 0 in
   {
     fp = fp;
@@ -45,9 +45,9 @@ let ptr_resource (#a:Type) (ptr:B.pointer a) =
 
 let reveal_ptr ()
   : Lemma ((forall a (ptr:B.pointer a) .{:pattern as_loc (fp (ptr_resource ptr))} 
-             as_loc (fp (ptr_resource ptr)) == B.loc_buffer ptr) /\
+             as_loc (fp (ptr_resource ptr)) == B.loc_addr_of_buffer ptr) /\
            (forall a (ptr:B.pointer a) h .{:pattern inv (ptr_resource ptr) h} 
-             inv (ptr_resource ptr) h <==> B.live h ptr) /\
+             inv (ptr_resource ptr) h <==> B.live h ptr /\ B.freeable ptr) /\
            (forall a (ptr:B.pointer a) h .{:pattern sel (ptr_view ptr) h} 
              sel (ptr_view ptr) h == Seq.index (B.as_seq h ptr) 0)) = 
   ()
@@ -56,8 +56,8 @@ let reveal_ptr ()
 
 let ptr_read (#a:Type)
              (ptr:B.pointer a)
-             (_:unit)
-           : RST a (ptr_resource ptr) 
+           : RST a (ptr_resource ptr)
+                   (fun _ -> ptr_resource ptr)
                    (fun _ -> True)
                    (fun h0 x h1 -> 
                       sel (ptr_view ptr) h0 == x /\ 
@@ -68,8 +68,8 @@ let ptr_read (#a:Type)
 let ptr_write (#a:Type)
               (ptr:B.pointer a)
               (x:a)
-              (_:unit)
             : RST unit (ptr_resource ptr)
+                       (fun _ -> ptr_resource ptr)
                        (fun _ -> True)
                        (fun _ _ h1 -> 
                           sel (ptr_view ptr) h1 == x) =
@@ -77,59 +77,72 @@ let ptr_write (#a:Type)
   reveal_modifies ();
   ptr *= x
 
-(* Scoped allocation of pointer resources *)
 
-(* Another (currently assumed) lemmas about loc_not_unused_in *)
-assume val lemma_loc_not_unused_in_fresh_frame (l:B.loc) (h0 h1:HS.mem) 
-  : Lemma (requires (B.loc_includes (B.loc_not_unused_in h0) l /\ HS.fresh_frame h0 h1))
-          (ensures  (B.loc_includes (B.loc_not_unused_in h1) l)) 
 
-assume val lemma_loc_not_unused_in_popped (l:B.loc) (h0 h1:HS.mem) 
-  : Lemma (requires (B.loc_includes (B.loc_not_unused_in h0) l /\ HS.popped h0 h1))
-          (ensures  (B.loc_includes (B.loc_not_unused_in h1) l)) 
+(* Unscoped allocation and deallocation of pointer resources *)
+
+let ptr_alloc (#a:Type)
+              (init:a)
+            : RST (B.pointer a) (empty_resource)
+                                (fun ptr -> ptr_resource ptr)
+                                (fun _ -> True)
+                                (fun _ ptr h1 -> 
+                                   sel (ptr_view ptr) h1 == init) =
+  reveal_rst_inv ();
+  reveal_modifies ();
+  B.malloc HS.root init 1ul
+
+let ptr_free (#a:Type)
+             (ptr:B.pointer a)
+           : RST unit (ptr_resource ptr)
+                      (fun ptr -> empty_resource)
+                      (fun _ -> True)
+                      (fun _ ptr h1 -> True) =
+  reveal_rst_inv ();
+  reveal_modifies ();
+  B.free ptr
+
+(* Scoped allocation of (heap-allocated, freeable) pointer resources *)
 
 unfold
 let with_new_ptr_pre (res:resource) =
-  pre:r_pre res{(forall h0 h1.{:pattern pre h0; HS.fresh_frame h0 h1} 
-                   pre h0 /\ HS.fresh_frame h0 h1 ==> pre h1) /\
-                (forall h0 h1.{:pattern pre h0; B.modifies B.loc_none h0 h1} 
-                   pre h0 /\ B.modifies B.loc_none h0 h1 ==> pre h1)}
+  pre:r_pre res{forall h0 h1 . 
+                  pre h0 /\ 
+                  sel (view_of res) h0 == sel (view_of res) h1 
+                  ==> 
+                  pre h1}
 
 unfold
-let with_new_ptr_post (res:resource) (a:Type) =
-  post:r_post res a{(forall h0 h1 x h2.{:pattern B.modifies B.loc_none h0 h1; post h1 x h2} 
-                       B.modifies B.loc_none h0 h1 /\ post h1 x h2 ==> post h0 x h2) /\
-                    (forall h0 h1 x h2.{:pattern HS.fresh_frame h0 h1; post h1 x h2}
-                       rst_inv res h0 /\ HS.fresh_frame h0 h1 /\ post h1 x h2 ==> post h0 x h2) /\ 
-                    (forall h0 x h1 h2.{:pattern post h0 x h1; HS.popped h1 h2}
-                       post h0 x h1 /\ HS.popped h1 h2 /\ rst_inv res h2 ==> post h0 x h2)}
+let with_new_ptr_post (res0:resource) (a:Type) (res1:a -> resource) =
+  post:r_post res0 a res1{forall h0 h1 x h2 h3 . 
+                            sel (view_of res0) h0 == sel (view_of res0) h1 /\
+                            post h1 x h2 /\
+                            sel (view_of (res1 x)) h2 == sel (view_of (res1 x)) h3 
+                            ==>
+                            post h0 x h3}
 
 let with_new_ptr (#res:resource)
                  (#a:Type)
                  (init:a)
                  (#b:Type)
                  (#pre:with_new_ptr_pre res)
-                 (#post:with_new_ptr_post res b)
-                 (f:(ptr:B.pointer a -> RST b (res <*> (ptr_resource ptr)) 
+                 (#post:with_new_ptr_post res b (fun _ -> res))
+                 (f:(ptr:B.pointer a -> RST b (res <*> (ptr_resource ptr))
+                                              (fun _ -> res <*> (ptr_resource ptr))
                                               (fun h -> pre h /\ sel (ptr_view ptr) h == init) 
-                                              post)) 
-               : RST b res pre post = 
-  reveal_rst_inv ();
-  reveal_modifies ();
-  reveal_view ();
+                                              (post))) 
+               : RST b res (fun _ -> res) pre post = 
   reveal_star ();
-  reveal_ptr ();
-  let h0 = get () in
-  HST.push_frame ();
-  let h1 = get () in
-  lemma_loc_not_unused_in_fresh_frame (as_loc (fp res)) h0 h1;
-  let ptr = B.alloca init 1ul in
-  let h2 = get () in
-  lemma_loc_not_unused_in_modifies (as_loc (fp res)) h1 h2;
-  let x = f ptr in
-  let h3 = get () in
-  HST.pop_frame ();
-  let h4 = get () in
-  B.modifies_fresh_frame_popped h0 h1 (as_loc (fp (res <*> (ptr_resource ptr)))) h3 h4;
-  lemma_loc_not_unused_in_popped (as_loc (fp res)) h3 h4;
+  let ptr = 
+    rst_frame 
+      #res #_ #_ 
+      #(fun ptr -> res <*> ptr_resource ptr)
+      res 
+      (fun _ -> ptr_alloc init) in
+  let x = f ptr in 
+  rst_frame
+    #(res <*> ptr_resource ptr) #_ #_ 
+    #(fun _ -> res)
+    res 
+    (fun _ -> ptr_free ptr);
   x
